Prove steps_io_event_thm with one cheat remaining

pancake/proofs/time_to_panProofScript.sml
@@ -612,6 +612,15 @@ Definition wait_time_locals1_def:
         nst < wt + ist
 End
 
+
+Definition input_stime_rel_def:
+  (input_stime_rel NONE _ _ ⇔ T) ∧
+  (input_stime_rel (SOME (wt:num)) ist st ⇔
+   ist ≤ st ∧
+   st < ist + wt)
+End
+
+
 (*
 Definition wait_time_locals_def:
   wait_time_locals (:α) fm swt ffi =
@@ -719,8 +728,27 @@ Definition event_inv_def:
     FLOOKUP fm «event» = SOME (ValWord 0w)
 End
 
+(*
+  step_delay: wakeup_shape t.locals s.waitTime ist
+  step_input:  wakeup_shape t.locals s.waitTime ist ∧
+  step_output:
+*)
+
+(*
+step_delay: wait_time_locals1 (:α) t'.locals s'.waitTime ist
+                        (FST (t.ffi.ffi_state cycles))
+step_input:
+step_output:
+
+*)
+
+(*
+  wakeup_shape does not stay invariant as such
+*)
+
+
 Definition assumptions_def:
-  assumptions prog n ist s (t:('a,time_input) panSem$state) ⇔
+  assumptions prog n s (t:('a,time_input) panSem$state) ⇔
     state_rel (clksOf prog) (out_signals prog) s t ∧
     code_installed t.code prog ∧
     well_formed_code prog t.code ∧
@@ -728,7 +756,6 @@ Definition assumptions_def:
     good_dimindex (:'a) ∧
     ~MEM "get_time_input" (MAP explode (out_signals prog)) ∧
     event_inv t.locals ∧
-    wakeup_shape t.locals s.waitTime ist ∧
     task_ret_defined t.locals (nClks prog)
 End
 
@@ -742,13 +769,14 @@ Definition evaluations_def:
      | LAction act =>
         (case act of
          | Input i =>
-             evaluate_input prog i ist s st t lbls sts
+             evaluate_input prog i s st t lbls sts
          | Output os =>
-             evaluate_output prog os ist st t lbls sts)) ∧
+             evaluate_output prog os st t lbls sts)) ∧
 
   (evaluate_delay prog d ist s st (t:('a,time_input) panSem$state) lbls sts ⇔
    ∀cycles.
      delay_rep d t.ffi.ffi_state cycles ∧
+     wakeup_shape t.locals s.waitTime ist ∧
      wakeup_rel t.locals s.waitTime ist t.ffi.ffi_state cycles ∧
      mem_read_ffi_results (:α) t.ffi.ffi_state cycles ∧
      t.ffi.io_events ≠ [] ∧
@@ -775,8 +803,9 @@ Definition evaluations_def:
        task_ret_defined nt.locals (nClks prog) ∧
        evaluations prog lbls sts ist st nt) ∧
 
-  (evaluate_input prog i ist s st (t:('a,time_input) panSem$state) lbls sts ⇔
-   input_stime_rel s.waitTime ist (FST (t.ffi.ffi_state 0)) ∧
+  (evaluate_input prog i s st (t:('a,time_input) panSem$state) lbls sts ⇔
+   wakeup_shape t.locals s.waitTime (FST (t.ffi.ffi_state 0)) ∧
+   input_stime_rel s.waitTime (FST (t.ffi.ffi_state 0)) (FST (t.ffi.ffi_state 0)) ∧
    input_rel t.locals i (next_ffi t.ffi.ffi_state) ∧
    mem_read_ffi_results (:α) t.ffi.ffi_state 1 ⇒
    ∃ck nt.
@@ -806,7 +835,7 @@ Definition evaluations_def:
      task_ret_defined nt.locals (nClks prog) ∧
      evaluations prog lbls sts (FST (t.ffi.ffi_state 0)) st nt) ∧
 
-  (evaluate_output prog os ist st (t:('a,time_input) panSem$state) lbls sts ⇔
+  (evaluate_output prog os st (t:('a,time_input) panSem$state) lbls sts ⇔
    output_rel t.locals t.ffi.ffi_state ⇒
    ∃ck nt.
      (∀ck_extra.
@@ -838,145 +867,6 @@ Termination
   cheat
 End
 
-(*
-Definition action_rel_def:
-  (action_rel (Input i) s (t:('a,time_input) panSem$state) ffi ⇔
-    input_rel t.locals i (next_ffi t.ffi.ffi_state) ∧
-    mem_read_ffi_results (:α) t.ffi.ffi_state 1 ∧
-    ffi = next_ffi t.ffi.ffi_state) ∧
-  (action_rel (Output os) s t ffi ⇔
-    output_rel t.locals t.ffi.ffi_state ∧
-    ffi = t.ffi.ffi_state)
-End
-
-
-Definition ffi_rel_def:
-  (ffi_rel (LDelay d) s (t:('a,time_input) panSem$state) ffi =
-   ∃cycles.
-     delay_rep d t.ffi.ffi_state cycles ∧
-     wakeup_rel t.locals s.waitTime t.ffi.ffi_state cycles ∧
-     mem_read_ffi_results (:α) t.ffi.ffi_state cycles ∧
-     ffi = nexts_ffi cycles t.ffi.ffi_state ∧
-     t.ffi.io_events ≠ [] ∧
-     EL 0 (io_event_dest (:α) t.be (LAST t.ffi.io_events)) =
-     FST (t.ffi.ffi_state 0)) ∧
-  (ffi_rel (LAction act) s t ffi =
-     action_rel act s t ffi)
-End
-
-Definition ffi_rels_def:
-  (ffi_rels prog [] s (t:('a,time_input) panSem$state) ⇔ T) ∧
-  (ffi_rels prog (label::labels) s t ⇔
-   ∃ffi.
-     ffi_rel label s t ffi ∧
-     ∀s' (t':('a,time_input) panSem$state) m n.
-       step prog label m n s s' ∧
-       t'.ffi.ffi_state = ffi ⇒
-       ffi_rels prog labels s' t')
-End
-
-(* TODO: change - to + :
-         SUM (n::ns) + 1 = LENGTH ios *)
-Definition decode_ios_def:
-  (decode_ios (:α) be [] [] ios ⇔ LENGTH ios = 1) ∧
-  (decode_ios (:α) be (lbl::lbls) (n::ns) ios ⇔
-   SUM (n::ns) = LENGTH ios - 1 ∧
-   (case lbl of
-    | LDelay d =>
-        (if n = 0
-         then d = 0 ∧ decode_ios (:α) be lbls ns ios
-         else
-           let
-             m' = EL 0 (io_event_dest (:α) be (HD ios));
-             nios = TAKE n (TL ios);
-             obs_ios = decode_io_events (:'a) be nios;
-             m = THE (to_delay (EL (LENGTH obs_ios - 1) obs_ios))
-           in
-             d = m - m' ∧
-             decode_ios (:α) be lbls ns (DROP n ios))
-    | LAction act =>
-        (n = 1 ∧
-         decode_ios (:α) be lbls ns (DROP 1 ios) ∧
-         (case act of
-          | Input i =>
-              let
-                obs_io = decode_io_event (:α) be (EL 1 ios)
-              in
-                Input i = THE (to_input obs_io)
-          | Output os =>
-              decode_io_event (:α) be (EL 1 ios) = ObsOutput os))))
-End
-
-
-Definition gen_max_times_def:
-  (gen_max_times [] n ns = ns) ∧
-  (gen_max_times (lbl::lbls) n ns =
-   n ::
-   let m =
-       case lbl of
-       | LDelay d => d + n
-       | LAction _ => n
-   in
-   gen_max_times lbls m ns)
-End
-
-Definition init_clocks_def:
-  init_clocks fm clks ⇔
-    EVERY
-      (λck. FLOOKUP fm ck = SOME (0:num)) clks
-End
-
-Definition init_ffi_def:
-  init_ffi (f:num -> num # num) ⇔
-    f 0 =  f 1 ∧
-    SND (f 0) = 0
-End
-
-
-Definition locals_before_start_ctrl_def:
-  locals_before_start_ctrl prog wt ffi =
-  FEMPTY |+ («loc» ,ValLabel (toString (FST (ohd prog)))) |+
-         («waitSet» ,
-          ValWord (case wt of NONE => 1w | SOME v => 0w)) |+
-         («event» ,ValWord 0w) |+ («isInput» ,ValWord 1w) |+
-         («wakeUpAt» ,ValWord 0w) |+ («sysTime» ,ValWord 0w) |+
-         («ptr1» ,ValWord 0w) |+ («len1» ,ValWord 0w) |+
-         («ptr2» ,ValWord ffiBufferAddr) |+
-         («len2» ,ValWord ffiBufferSize) |+
-         («taskRet» ,
-          Struct
-          [Struct (emptyVals (nClks prog)); ValWord 0w; ValWord 0w;
-           ValLabel (toString (FST (ohd prog)))]) |+
-         («clks» ,Struct (emptyVals (nClks prog))) |+
-         («sysTime» ,ValWord (n2w (FST ffi))) |+
-         («event» ,ValWord (n2w (SND ffi))) |+
-         («isInput» ,ValWord 1w) |+
-         («clks» ,
-          Struct
-          (REPLICATE (nClks prog)
-           (ValWord (n2w (FST ffi))))) |+
-         («wakeUpAt» ,
-          ValWord
-          (n2w
-           (case wt of
-              NONE => FST ffi
-            | SOME n => n + FST ffi)))
-End
-
-Definition ffi_rels_after_init_def:
-  ffi_rels_after_init prog labels st (t:('a,time_input) panSem$state) ⇔
-  ∀bytes.
-    read_bytearray ffiBufferAddr (w2n (ffiBufferSize:'a word))
-                   (mem_load_byte t.memory t.memaddrs t.be) = SOME bytes ⇒
-    ffi_rels prog labels st
-             (t with
-              <|locals :=
-                locals_before_start_ctrl prog st.waitTime (t.ffi.ffi_state 0);
-                memory :=
-                mem_call_ffi (:α) t.memory t.memaddrs t.be t.ffi.ffi_state;
-                ffi := ffi_call_ffi (:α) t.be t.ffi bytes|>)
-End
-*)
 
 Theorem length_get_bytes:
   ∀w be.
@@ -5904,15 +5794,8 @@ Proof
   metis_tac [mod_greater_neq1]
 QED
 
-Definition input_stime_rel_def:
-  (input_stime_rel NONE _ _ ⇔ T) ∧
-  (input_stime_rel (SOME (wt:num)) ist st ⇔
-   ist ≤ st ∧
-   st < ist + wt)
-End
-
 Theorem step_input:
-  !prog i m n s s' (t:('a,time_input) panSem$state) ist.
+  !prog i m n s s' (t:('a,time_input) panSem$state).
     step prog (LAction (Input i)) m n s s' ∧
     m = dimword (:α) - 1 ∧
     n = FST (t.ffi.ffi_state 0) ∧
@@ -7466,8 +7349,8 @@ QED
 Theorem steps_thm:
   ∀labels prog n ist st sts (t:('a,time_input) panSem$state).
     steps prog labels (dimword (:α) - 1) n st sts ∧
-    assumptions prog n ist st t ⇒
-      evaluations prog labels sts  ist st t
+    assumptions prog n st t ⇒
+     evaluations prog labels sts ist st t
 Proof
   Induct
   >- (
@@ -7503,7 +7386,8 @@ Proof
     gs [panSemTheory.dec_clock_def] >>
     qexists_tac ‘t'' with clock := t''.clock + 1’ >>
     conj_tac
-    >- rw [] >> gs [] >>
+    >- rw [] >>
+    gs [] >>
     conj_asm1_tac
     >- gs [state_rel_def] >>
     gs [] >>
@@ -7533,10 +7417,11 @@ Proof
     conj_asm1_tac
     >- gs [task_ret_defined_def] >>
     last_x_assum match_mp_tac >>
-    gs [nexts_ffi_def, delay_rep_def] >>
+    gs [nexts_ffi_def, delay_rep_def]) >>
+    (*
     gvs [wakeup_shape_def] >>
     qexists_tac ‘wt'’ >> gs [] >>
-    gs [step_cases, mkState_def]) >>
+    gs [step_cases, mkState_def]) >> *)
   cases_on ‘i’ >>
   gs []
   >- (
@@ -7547,7 +7432,7 @@ Proof
     rw [] >>
     drule step_input >>
     gs [] >>
-    disch_then (qspecl_then [‘t’, ‘ist’] mp_tac) >>
+    disch_then (qspecl_then [‘FST (t.ffi.ffi_state 0)’, ‘t’] mp_tac) >>
     impl_tac
     >- (
       gs [timeSemTheory.step_cases] >>
@@ -7577,17 +7462,16 @@ Proof
       rw [] >>
       drule evaluate_add_clock_eq >>
       gs []) >>
-    conj_asm1_tac
+    cases_on ‘h'.waitTime’ >>
+    gs [wait_time_locals1_def]
     >- (
-      cases_on ‘h'.waitTime’ >>
-      gs [wait_time_locals1_def]
-      >- (
-       qexists_tac ‘0’ >>
-       gs [good_dimindex_def, dimword_def]) >>
-      qexists_tac ‘x’ >>
-      gs [step_cases] >>
-      drule pick_term_dest_eq >>
-      gs []) >>
+      qexists_tac ‘0’ >>
+      gs [good_dimindex_def, dimword_def]) >>
+    qexists_tac ‘x’ >>
+    gs [step_cases] >>
+    drule pick_term_dest_eq >>
+    gs []) >>
+  (*
     last_x_assum match_mp_tac >>
     gs [] >>
     gs [wakeup_shape_def] >>
@@ -7599,7 +7483,7 @@ Proof
     gs [] >>
     gs [step_cases] >>
     drule pick_term_dest_eq >>
-    gs []) >>
+    gs []) >> *)
   (* output step *)
   gs [steps_def] >>
   gs [assumptions_def, event_inv_def, evaluations_def, event_inv_def] >>
@@ -7625,31 +7509,161 @@ Proof
     rw [] >>
     drule evaluate_add_clock_eq >>
     gs []) >>
-  conj_asm1_tac
-  >- (
-    cases_on ‘h'.waitTime’ >>
-    gs [wait_time_locals1_def]
-    >- (
-      qexists_tac ‘0’ >>
-      gs [good_dimindex_def, dimword_def]) >>
-    qexists_tac ‘x’ >>
-    gs [] >>
-    gs [step_cases] >>
-    drule pick_term_dest_eq >>
-    gs []) >>
-  last_x_assum match_mp_tac >>
-  gs [] >>
-  gs [wakeup_shape_def] >>
-  cases_on ‘h'.waitTime’ >> gs []
+  cases_on ‘h'.waitTime’ >>
+  gs [wait_time_locals1_def]
   >- (
     qexists_tac ‘0’ >>
-    gs []) >>
+    gs [good_dimindex_def, dimword_def]) >>
   qexists_tac ‘x’ >>
   gs [] >>
   gs [step_cases] >>
   drule pick_term_dest_eq >>
   gs []
 QED
+
+
+Definition action_rel_def:
+  (action_rel (Input i) s (t:('a,time_input) panSem$state) ffi ⇔
+   wakeup_shape t.locals s.waitTime (FST (t.ffi.ffi_state 0)) ∧
+    input_stime_rel s.waitTime (FST (t.ffi.ffi_state 0)) (FST (t.ffi.ffi_state 0)) ∧
+    input_rel t.locals i (next_ffi t.ffi.ffi_state) ∧
+    mem_read_ffi_results (:α) t.ffi.ffi_state 1 ∧
+    ffi = next_ffi t.ffi.ffi_state) ∧
+  (action_rel (Output os) s t ffi ⇔
+    output_rel t.locals t.ffi.ffi_state ∧
+    ffi = t.ffi.ffi_state)
+End
+
+
+Definition ffi_rel_def:
+  (ffi_rel (LDelay d) s (t:('a,time_input) panSem$state) ist ffi =
+   ∃cycles.
+     delay_rep d t.ffi.ffi_state cycles ∧
+     wakeup_shape t.locals s.waitTime ist ∧
+     wakeup_rel t.locals s.waitTime ist t.ffi.ffi_state cycles ∧
+     mem_read_ffi_results (:α) t.ffi.ffi_state cycles ∧
+     ffi = nexts_ffi cycles t.ffi.ffi_state ∧
+     t.ffi.io_events ≠ [] ∧
+     EL 0 (io_event_dest (:α) t.be (LAST t.ffi.io_events)) =
+     FST (t.ffi.ffi_state 0)) ∧
+  (ffi_rel (LAction act) s t ist ffi ⇔
+   ist = (FST (t.ffi.ffi_state 0)) ∧
+   action_rel act s t ffi)
+End
+
+Definition ffi_rels_def:
+  (ffi_rels prog [] s (t:('a,time_input) panSem$state) ist ⇔ T) ∧
+  (ffi_rels prog (label::labels) s t ist ⇔
+   ∃ffi.
+     ffi_rel label s t ist ffi ∧
+     ∀s' (t':('a,time_input) panSem$state) m n.
+       step prog label m n s s' ∧
+       t'.ffi.ffi_state = ffi ⇒
+       ffi_rels prog labels s' t' ist)
+End
+
+(* TODO: change - to + :
+         SUM (n::ns) + 1 = LENGTH ios *)
+Definition decode_ios_def:
+  (decode_ios (:α) be [] [] ios ⇔ LENGTH ios = 1) ∧
+  (decode_ios (:α) be (lbl::lbls) (n::ns) ios ⇔
+   SUM (n::ns) = LENGTH ios - 1 ∧
+   (case lbl of
+    | LDelay d =>
+        (if n = 0
+         then d = 0 ∧ decode_ios (:α) be lbls ns ios
+         else
+           let
+             m' = EL 0 (io_event_dest (:α) be (HD ios));
+             nios = TAKE n (TL ios);
+             obs_ios = decode_io_events (:'a) be nios;
+             m = THE (to_delay (EL (LENGTH obs_ios - 1) obs_ios))
+           in
+             d = m - m' ∧
+             decode_ios (:α) be lbls ns (DROP n ios))
+    | LAction act =>
+        (n = 1 ∧
+         decode_ios (:α) be lbls ns (DROP 1 ios) ∧
+         (case act of
+          | Input i =>
+              let
+                obs_io = decode_io_event (:α) be (EL 1 ios)
+              in
+                Input i = THE (to_input obs_io)
+          | Output os =>
+              decode_io_event (:α) be (EL 1 ios) = ObsOutput os))))
+End
+
+
+Definition gen_max_times_def:
+  (gen_max_times [] n ns = ns) ∧
+  (gen_max_times (lbl::lbls) n ns =
+   n ::
+   let m =
+       case lbl of
+       | LDelay d => d + n
+       | LAction _ => n
+   in
+   gen_max_times lbls m ns)
+End
+
+Definition init_clocks_def:
+  init_clocks fm clks ⇔
+    EVERY
+      (λck. FLOOKUP fm ck = SOME (0:num)) clks
+End
+
+Definition init_ffi_def:
+  init_ffi (f:num -> num # num) ⇔
+    f 0 =  f 1 ∧
+    SND (f 0) = 0
+End
+
+
+Definition locals_before_start_ctrl_def:
+  locals_before_start_ctrl prog wt ffi =
+  FEMPTY |+ («loc» ,ValLabel (toString (FST (ohd prog)))) |+
+         («waitSet» ,
+          ValWord (case wt of NONE => 1w | SOME v => 0w)) |+
+         («event» ,ValWord 0w) |+ («isInput» ,ValWord 1w) |+
+         («wakeUpAt» ,ValWord 0w) |+ («sysTime» ,ValWord 0w) |+
+         («ptr1» ,ValWord 0w) |+ («len1» ,ValWord 0w) |+
+         («ptr2» ,ValWord ffiBufferAddr) |+
+         («len2» ,ValWord ffiBufferSize) |+
+         («taskRet» ,
+          Struct
+          [Struct (emptyVals (nClks prog)); ValWord 0w; ValWord 0w;
+           ValLabel (toString (FST (ohd prog)))]) |+
+         («clks» ,Struct (emptyVals (nClks prog))) |+
+         («sysTime» ,ValWord (n2w (FST ffi))) |+
+         («event» ,ValWord (n2w (SND ffi))) |+
+         («isInput» ,ValWord 1w) |+
+         («clks» ,
+          Struct
+          (REPLICATE (nClks prog)
+           (ValWord (n2w (FST ffi))))) |+
+         («wakeUpAt» ,
+          ValWord
+          (n2w
+           (case wt of
+              NONE => FST ffi
+            | SOME n => n + FST ffi)))
+End
+
+Definition ffi_rels_after_init_def:
+  ffi_rels_after_init prog labels st (t:('a,time_input) panSem$state) ⇔
+  ∀bytes.
+    read_bytearray ffiBufferAddr (w2n (ffiBufferSize:'a word))
+                   (mem_load_byte t.memory t.memaddrs t.be) = SOME bytes ⇒
+    ffi_rels prog labels st
+             (t with
+              <|locals :=
+                locals_before_start_ctrl prog st.waitTime (t.ffi.ffi_state 0);
+                memory :=
+                mem_call_ffi (:α) t.memory t.memaddrs t.be t.ffi.ffi_state;
+                ffi := ffi_call_ffi (:α) t.be t.ffi bytes|>)
+             (FST (t.ffi.ffi_state 0))
+End
 
 
 Theorem decode_ios_length_eq_sum:
@@ -7694,10 +7708,10 @@ End
 
 
 Theorem steps_io_event_thm:
-  ∀labels prog n st sts (t:('a,time_input) panSem$state).
+  ∀labels prog n st sts (t:('a,time_input) panSem$state) ist.
     steps prog labels (dimword (:α) - 1) n st sts ∧
     assumptions prog n st t ∧
-    ffi_rels prog labels st t ∧
+    ffi_rels prog labels st t ist ∧
     sum_delays (:α) labels t.ffi.ffi_state ⇒
     ∃ck t' ns ios.
       evaluate (time_to_pan$always (nClks prog), t with clock := t.clock + ck) =
@@ -7714,9 +7728,10 @@ Proof
   rw [] >>
   gs [] >>
   drule_all steps_thm >>
+  disch_then (qspec_then ‘ist’ mp_tac) >>
   strip_tac >>
   rpt (pop_assum mp_tac) >>
-  MAP_EVERY qid_spec_tac [‘t’, ‘sts’, ‘st’, ‘n’, ‘prog’, ‘labels'’] >>
+  MAP_EVERY qid_spec_tac [‘ist’, ‘t’, ‘sts’, ‘st’, ‘n’, ‘prog’, ‘labels'’] >>
   Induct
   >- (
     rw [] >>
@@ -7753,6 +7768,8 @@ Proof
       gs [] >>
       ‘FLOOKUP t.locals «waitSet» = SOME (ValWord 0w)’ by
         gs [assumptions_def, state_rel_def, equivs_def, active_low_def] >>
+
+
       drule step_wait_delay_eval_wait_not_zero >>
       impl_tac
       >- (
@@ -7761,7 +7778,7 @@ Proof
         pairarg_tac >> gs [] >>
         qexists_tac ‘dimword (:α) − 2’ >>
         gs [] >>
-        gs [wait_time_locals_def] >>
+        gs [wait_time_locals1_def] >>
         qexists_tac ‘st' + wt’ >>
         gs []) >>
       gs []) >>
@@ -7916,7 +7933,7 @@ Proof
     gs [] >>
     strip_tac >>
     last_x_assum drule >>
-    disch_then (qspec_then ‘nt’ mp_tac) >>
+    disch_then (qspecl_then [‘nt’, ‘ist’] mp_tac) >>
     impl_tac
     >- (
       gs [assumptions_def] >>
@@ -8020,10 +8037,10 @@ Proof
     impl_tac >- gs [] >>
     strip_tac >>
     last_x_assum drule >>
-    disch_then (qspec_then ‘nt’ mp_tac) >>
+    disch_then (qspecl_then [‘nt’, ‘ist’] mp_tac) >>
     impl_tac
     >- (
-      gs [assumptions_def] >>
+      gvs [assumptions_def] >>
       gs [nexts_ffi_def, input_rel_def] >>
       qpat_x_assum ‘state_rel _ _ _ t’ assume_tac >>
       gs [state_rel_def] >>
@@ -8036,6 +8053,7 @@ Proof
         gs [] >>
         gs [input_rel_def, next_ffi_def]) >>
       gs [next_ffi_def] >>
+      strip_tac >>
       cases_on ‘evaluate (always (nClks prog),t)’ >>
       gs [] >>
       drule evaluate_add_clock_eq >>
@@ -8087,7 +8105,7 @@ Proof
   impl_tac >- gs [] >>
   strip_tac >>
   last_x_assum drule >>
-  disch_then (qspec_then ‘nt’ mp_tac) >>
+  disch_then (qspecl_then [‘nt’, ‘ist’] mp_tac) >>
   impl_tac
   >- (
     gs [assumptions_def] >>
